dafny/project/BloodType.dfy
@@ -1,5 +1,5 @@
 // The datatype to store the valuable information of ID, expirayDate, arrivalDate of the bloodBag (in that order)
-datatype BloodBags<B> = Leaf(B, B, B) | Node(B, B, B, BloodBags<B>)
+datatype BloodBags<B, C> = Leaf(B, B, B, C) | Node(B, B, B, BloodBags<B, C>)
 
 class BloodType 
 {
@@ -7,8 +7,8 @@ class BloodType
     var bloodType: string;
     var lowest: int;
     var quantity: int;
-    var Leaf1:BloodBags<int>; 
-    var t1:BloodBags<int>;
+    var temp1:BloodBags<int, string>; 
+    var temp2:BloodBags<int, string>; 
 
     predicate ValidBT()
     reads this
@@ -19,14 +19,31 @@ class BloodType
         (bloodType == "A" || bloodType == "B" || bloodType == "O" || bloodType == "AB") 
     }
     
-    constructor()
+    constructor(bloodtype: string, critical: int)
+    requires critical >= 0 
+    requires bloodtype == "A" || bloodtype == "B" || bloodtype == "O" || bloodtype == "AB"
     ensures ValidBT()
-    ensures fresh(footprint - old(footprint))
-    modifies this, footprint
+    modifies this
     {
         bloodType := bloodtype;
         lowest := critical;
         quantity := 0;
+        temp1 := Leaf(0, 0, 0, " ");
+        footprint := {this};
     }
-    
+
+    method addBloodBag(ID: int, expDate: int, arvDate: int) returns(test: bool)
+    requires ValidBT()
+    ensures ValidBT()
+    modifies this
+    {
+        var node:BloodBags<int> := Node(ID, expDate, arvDate, temp1);
+        temp1 := node;
+    }
+
+}
+
+method Main() {
+    var bloodyType := new BloodType();
+
 }
