dafny/project/BloodTypeReal.dfy
@@ -1,14 +1,14 @@
-datatype BloodType<B> = Leaf(B, B, B) | Node(B, B, B, BloodType<B>)
+datatype BloodType<B, C> = Leaf(B, B, B, C) | Node(B, B, B, C, BloodType<B, C>)
 
-method Print(t:BloodType<int>) // BOTTOM-UP
+method Print(t:BloodType<int, string>) // BOTTOM-UP
 {
     match t
-        case Leaf(n, l, r) => print n, ' ', l, ' ', r, ' '; 
-        case Node(n,l,r,k) => { print n, ' ', l, ' ', r, ' '; Print(k); }
+        case Leaf(n, l, r, k) => print n, ' ', l, ' ', r, ' ', k, ' '; 
+        case Node(n,l,r,k, p) => { print n, ' ', l, ' ', r, ' ', k, ' '; Print(p); }
 }
 method Main(){
-    var Leaf1:BloodType<int> := Leaf(1, 2, 3);
-    var t1:BloodType<int> := Node(2, 7, 5, Leaf1);
+    var Leaf1:BloodType<int, string> := Leaf(1, 2, 3, "A");
+    var t1:BloodType<int, string> := Node(2, 7, 5, "B", Leaf1);
     Print(t1); print '\n'; 
 
 }
